theories/lang/memcpy.v
@@ -21,9 +21,9 @@ Notation "e1 <-{ n ',Σ' i } ! e2" :=
   (at level 80, n, i at next level,
    format "e1  <-{ n ,Σ  i }  ! e2") : expr_scope.
 
-Lemma wp_memcpy `{heapG Σ} E l1 l2 vl1 vl2 q n:
+Lemma wp_memcpy `{heapG Σ} E l1 l2 vl1 vl2 q (n : Z):
   ↑heapN ⊆ E →
-  length vl1 = n → length vl2 = n →
+  Z.of_nat (length vl1) = n → Z.of_nat (length vl2) = n →
   {{{ heap_ctx ∗ l1 ↦∗ vl1 ∗ l2 ↦∗{q} vl2 }}}
     #l1 <-{n} !#l2 @ E
   {{{ RET #(); l1 ↦∗ vl2 ∗ l2 ↦∗{q} vl2 }}}.
@@ -32,11 +32,10 @@ Proof.
   iLöb as "IH" forall (n l1 l2 vl1 vl2 Hvl1 Hvl2). wp_rec. wp_op=> ?; wp_if.
   - iApply "HΦ". assert (n = O) by lia; subst.
     destruct vl1, vl2; try discriminate. by iFrame.
-  - destruct vl1 as [|v1 vl1], vl2 as [|v2 vl2], n as [|n]; try discriminate.
-    revert Hvl1 Hvl2. intros [= Hvl1] [= Hvl2]; rewrite !heap_mapsto_vec_cons.
+  - destruct vl1 as [|v1 vl1], vl2 as [|v2 vl2], n as [|n|]; try discriminate.
+    revert Hvl1 Hvl2. intros [= Hvl1] [= Hvl2]; rewrite !heap_mapsto_vec_cons. subst n.
     iDestruct "Hl1" as "[Hv1 Hl1]". iDestruct "Hl2" as "[Hv2 Hl2]".
-    wp_read; wp_write. replace (Z.pos (Pos.of_succ_nat n)) with (n+1) by lia.
-    do 3 wp_op. rewrite Z.add_simpl_r.
-    iApply ("IH" with "[%] [%] Hl1 Hl2"); try done.
+    Local Opaque Zminus.
+    wp_read; wp_write. do 3 wp_op. iApply ("IH" with "[%] [%] Hl1 Hl2"); [lia..|].
     iIntros "!> [Hl1 Hl2]"; iApply "HΦ"; by iFrame.
 Qed.
